src/Helpers/FunMap.v
@@ -1,0 +1,65 @@
+Require Import Helpers.
+Require Import FunctionalExtensionality.
+
+Set Implicit Arguments.
+
+
+Section FunMap.
+
+  Variable A : Type.
+  Variable V : Type.
+  Context {Aeq : EqualDec A}.
+
+  Definition funmap := A -> V.
+
+  Definition fupd (a : A) (v : V) (m : funmap) : funmap :=
+    fun a' => if a == a' then v else m a'.
+
+  Theorem fupd_eq : forall a v m,
+    fupd a v m a = v.
+  Proof.
+    unfold fupd; intros.
+    destruct (a == a); congruence.
+  Qed.
+
+  Theorem fupd_ne : forall a a' v m,
+    a <> a' ->
+    fupd a v m a' = m a'.
+  Proof.
+    unfold fupd; intros.
+    destruct (a == a'); congruence.
+  Qed.
+
+  Theorem fupd_fupd_eq : forall a v v' m,
+    fupd a v (fupd a v' m) = fupd a v m.
+  Proof.
+    unfold fupd; intros.
+    eapply functional_extensionality; intros.
+    destruct (a == x); congruence.
+  Qed.
+
+  Theorem fupd_fupd_ne : forall a v a' v' m,
+    a <> a' ->
+    fupd a v (fupd a' v' m) = fupd a' v' (fupd a v m).
+  Proof.
+    unfold fupd; intros.
+    eapply functional_extensionality; intros.
+    destruct (a == x); destruct (a' == x); congruence.
+  Qed.
+
+  Theorem fupd_same : forall a v m,
+      m a = v ->
+      fupd a v m = m.
+  Proof.
+    intros.
+    extensionality a'; subst.
+    destruct (a == a'); subst.
+    rewrite fupd_eq; auto.
+    rewrite fupd_ne; auto.
+  Qed.
+
+End FunMap.
+
+Hint Rewrite fupd_eq : fupd.
+Hint Rewrite fupd_ne using congruence : fupd.
+Hint Rewrite fupd_fupd_eq using congruence : fupd.
